Rewrote proofs to make them reusable with other aux types

thys/MFODL_Monitor_Devel/Optimized_Agg.thy
@@ -9,11 +9,15 @@ datatype aggaux' = CntAux nat
 datatype aggaux = CntAux "nat agg_map" | SumAux "(nat \<times> event_data) agg_map" | MinAux "event_data table"
   | MaxAux "event_data table" | MedAux "event_data table"
 
-definition group_multiset where
-  "group_multiset k b f X = (let group = Set.filter (\<lambda>x. drop b x = k) X in
+definition group where [simp]:
+  "group k b X = Set.filter (\<lambda>x. drop b x = k) X"
+
+definition group_multiset where [simp]:
+  "group_multiset k b f X = (let group = group k b X in
                       (\<lambda>y. (y, ecard (Set.filter (\<lambda>x. meval_trm f x = y) group))) ` meval_trm f ` group)"
 
-definition valid_aggmap :: "(event_data list \<Rightarrow> 'a) \<Rightarrow> nat \<Rightarrow> Formula.trm \<Rightarrow> (event_data option list, 'a) mapping \<Rightarrow> event_data option list set \<Rightarrow> bool" where
+
+definition valid_aggmap :: "(event_data list \<Rightarrow> 'a) \<Rightarrow> nat \<Rightarrow> Formula.trm \<Rightarrow> (event_data option list, 'a) mapping \<Rightarrow> event_data option list set \<Rightarrow> bool" where [simp]:
   "valid_aggmap g b f m X \<longleftrightarrow> (\<forall>k. k \<in> (drop b) ` X \<longleftrightarrow> k \<in> Mapping.keys m) \<and>
                     (\<forall>k. k \<in> Mapping.keys m \<longrightarrow> Mapping.lookup m k = 
                     (let M = group_multiset k b f X
@@ -43,14 +47,16 @@ fun init_maggaux :: "aggargs \<Rightarrow> aggaux" where
     | Formula.Agg_Avg \<Rightarrow> SumAux Mapping.empty
     | Formula.Agg_Med \<Rightarrow> MedAux {})"
 
-fun insert_cnt :: "aggargs \<Rightarrow> nat agg_map \<Rightarrow> event_data tuple \<Rightarrow> nat agg_map" where
-  "insert_cnt args m t = (let group = drop (aggargs_b args) t 
+fun insert_cnt :: "aggargs \<Rightarrow>  event_data tuple \<Rightarrow> nat agg_map \<Rightarrow> nat agg_map" where
+  "insert_cnt args t m = (let group = drop (aggargs_b args) t 
                        in case (Mapping.lookup m group) of
                         Some i \<Rightarrow> Mapping.update group (i + 1) m
                       | None \<Rightarrow> Mapping.update group 1 m)"
 
-fun insert_sum :: "aggargs \<Rightarrow> event_data \<Rightarrow> (nat \<times> event_data) agg_map \<Rightarrow> event_data tuple \<Rightarrow> (nat \<times> event_data) agg_map" where
-  "insert_sum args y0 m t = (let group = drop (aggargs_b args) t;
+fun insert_sum :: "aggargs \<Rightarrow> event_data tuple \<Rightarrow> (nat \<times> event_data) agg_map \<Rightarrow> (nat \<times> event_data) agg_map" where
+  "insert_sum args t m = (let group = drop (aggargs_b args) t;
+                              aggtype = fst (aggargs_\<omega> args);
+                              y0 = (if aggtype = Formula.Agg_Sum then snd (aggargs_\<omega> args) else EInt 0);
                                          term = meval_trm (aggargs_f args) t
                                      in case (Mapping.lookup m group) of
                         Some (cnt, agg_sum) \<Rightarrow> Mapping.update group (cnt + 1, agg_sum + term) m
@@ -58,8 +64,8 @@ fun insert_sum :: "aggargs \<Rightarrow> event_data \<Rightarrow> (nat \<times> 
 
 fun insert_maggaux :: "aggargs \<Rightarrow> event_data table \<Rightarrow> aggaux \<Rightarrow> aggaux" where
   "insert_maggaux args data aux = (case aux of
-    CntAux m \<Rightarrow> CntAux (foldl (insert_cnt args) m (csorted_list_of_set data))
-  | SumAux m \<Rightarrow> let y0 = snd (aggargs_\<omega> args) in SumAux (foldl (insert_sum args y0) m (csorted_list_of_set data))
+    CntAux m \<Rightarrow> CntAux (Finite_Set.fold (insert_cnt args) m data)
+  | SumAux m \<Rightarrow> SumAux (Finite_Set.fold (insert_sum args) m data)
   | MinAux t \<Rightarrow> MinAux (t \<union> data)
   | MaxAux t \<Rightarrow> MaxAux (t \<union> data)
   | MedAux t \<Rightarrow> MedAux (t \<union> data))"
@@ -107,36 +113,45 @@ fun result_maggaux :: "aggargs \<Rightarrow> aggaux \<Rightarrow> event_data tab
   | MaxAux t \<Rightarrow> eval_aggargs \<lparr>aggargs_cols = cols, aggargs_n = n, aggargs_g0 = g0, aggargs_y = y, aggargs_\<omega> = \<omega>, aggargs_b = b, aggargs_f = f\<rparr> t
   | MedAux t \<Rightarrow> eval_aggargs \<lparr>aggargs_cols = cols, aggargs_n = n, aggargs_g0 = g0, aggargs_y = y, aggargs_\<omega> = \<omega>, aggargs_b = b, aggargs_f = f\<rparr> t)"
 
+lemma unique_term_multiset: "(t, y1) \<in> group_multiset k b f X \<Longrightarrow> y2 \<noteq> y1 \<Longrightarrow> (t, y2) \<notin> group_multiset k b f X"
+proof rule
+  assume term_in: "(t, y1) \<in> group_multiset k b f X" and not_eq: "y2 \<noteq> y1" and term_in_2: "(t, y2) \<in> group_multiset k b f X"
+  define group where [simp]: "group = Set.filter (\<lambda>x. drop b x = k) X"
+  have "y2 = ecard (Set.filter (\<lambda>x. meval_trm f x = t) group)" using term_in_2 by(auto simp: Let_def)
+  moreover have "y1 = ecard (Set.filter (\<lambda>x. meval_trm f x = t) group)" using term_in by(auto simp: Let_def)
+  ultimately show False using not_eq by auto
+qed
+
 lemma valid_init_maggaux_unfolded: "safe_aggargs \<lparr>aggargs_cols = cols, aggargs_n = n, aggargs_g0 = g0, aggargs_y = y, aggargs_\<omega> = \<omega>, aggargs_b = b, aggargs_f = f\<rparr> \<Longrightarrow> valid_maggaux \<lparr>aggargs_cols = cols, aggargs_n = n, aggargs_g0 = g0, aggargs_y = y, aggargs_\<omega> = \<omega>, aggargs_b = b, aggargs_f = f\<rparr> (init_maggaux \<lparr>aggargs_cols = cols, aggargs_n = n, aggargs_g0 = g0, aggargs_y = y, aggargs_\<omega> = \<omega>, aggargs_b = b, aggargs_f = f\<rparr>) {}"
-  by (cases "fst \<omega>") (auto simp add:valid_aggmap_def)
+  by (cases "fst \<omega>") auto
 
 lemma valid_init_maggaux: "safe_aggargs args \<Longrightarrow> valid_maggaux args (init_maggaux args) {}"
   using valid_init_maggaux_unfolded by (cases args) fast
 
-primrec iter_f :: "('a \<Rightarrow> 'b \<Rightarrow> 'b) \<Rightarrow> nat \<Rightarrow> 'a \<Rightarrow> 'b \<Rightarrow> 'b"
-  where
-    "iter_f f 0 t y0 = y0"
-  | "iter_f f (Suc n) t y0 = f t (iter_f f n t y0)"
+lemma insert_cnt_comm: "(insert_cnt args x \<circ> insert_cnt args y) m  = (insert_cnt args y \<circ> insert_cnt args x) m"
+  by (auto split:option.splits simp add: Let_def update_update(2) lookup_update') 
 
-lemma iter_f_comm: 
+lemma cmp_comm: 
   assumes commute_f: "comp_fun_commute f"
-  shows "iter_f f n1 t1 (iter_f f n2 t2 y0) = iter_f f n2 t2 (iter_f f n1 t1 y0)"
+  shows "(f t1 ^^ n1 \<circ> f t2 ^^ n2) y0 = (f t2 ^^ n2 \<circ> f t1 ^^ n1) y0" 
 proof(induction n1)
-  case 0
+case 0
   then show ?case by auto
 next
   case (Suc n)
-  then show ?case sorry
+  have aux1: "f t1 ((f t1 ^^ n) y0) = (f t1 ^^ n) (f t1 y0)" by (induction n) auto
+  moreover have "f t1 ((f t2 ^^ n2) ((f t1 ^^ n) y0)) = (f t2 ^^ n2) ((f t1 ^^ n) (f t1 y0))" 
+    using aux1 commute_f comp_fun_commute.fun_left_comm[of f t1 t2] by(induction n2) auto
+  ultimately show ?case using Suc by auto
 qed
-
 
 lemma fold_flatten_multiset: 
   assumes finite_m: "finite M"
   assumes commute_f: "comp_fun_commute f"
-  shows "fold f (flatten_multiset M) y0  = Finite_Set.fold (\<lambda> (t, m) y. iter_f f (the_enat m) t y) y0 M"
+  shows "fold f (flatten_multiset M) y0  = Finite_Set.fold (\<lambda> (t, m) y. ((f t) ^^ (the_enat m)) y) y0 M"
 proof -
-  interpret comp_fun_commute "\<lambda> (t, m) y. iter_f f (the_enat m) t y"
-    using iter_f_comm[of f] commute_f
+  interpret comp_fun_commute "\<lambda> (t, m) y. ((f t) ^^ (the_enat m)) y"
+    using cmp_comm[of f] commute_f
     by unfold_locales auto
   obtain c where c_def: "ID ccompare = Some (c :: (event_data \<times> enat) comparator)" 
     by (simp add: ID_def ccompare_prod_def ccompare_event_data_def ccompare_enat_def split:if_splits option.splits)
@@ -151,52 +166,168 @@ proof -
       by (auto simp add:flatten_multiset_def csorted_list_of_set_def c_def)
   next
     case (insert x F)
-    obtain t m where "x = (t, m)"
+    obtain t m where x_def: "x = (t, m)"
       by (cases x) auto
+    define xs where "xs = (linorder.sorted_list_of_set (le_of_comp c) F)"
+    have "fold f (concat (map (\<lambda>(x, c). replicate (the_enat c) x) (linorder.insort_key (le_of_comp c) (\<lambda>x. x) (t, m) xs))) y0
+       = (f t ^^ the_enat m) (fold f (concat (map (\<lambda>(x, c). replicate (the_enat c) x) xs)) y0)" 
+    proof(induction xs arbitrary: y0)
+      case Nil
+      then show ?case using linorder.insort_key.simps[OF c_class, of "(\<lambda>x. x)"] by (auto simp:xs_def)
+    next
+      case (Cons a as)
+      then show ?case 
+        using linorder.insort_key.simps[OF c_class, of "(\<lambda>x. x)"] cmp_comm[of f "the_enat m1"] 
+        by (auto simp:xs_def commute_f comp_fun_commute.comp_fun_commute fn_comm_power' fold_commute_apply)
+    qed
     then show ?case
-      using insert(1-2) insert(3)[symmetric] linorder.sorted_list_of_set_insert[OF c_class]
-      apply(simp add:flatten_multiset_def csorted_list_of_set_def c_def) sorry
+      using x_def insert linorder.sorted_list_of_set_insert[OF c_class]
+      by (simp add:flatten_multiset_def csorted_list_of_set_def c_def xs_def)
   qed
 qed
 
 lemma length_fold: "length xs = fold (\<lambda> _ n. n + 1) xs 0"
   by (induction xs) (auto simp:fold_commute_apply)
 
-lemma iter_f_len: "iter_f (\<lambda> _. Suc) m t y = y + m"
-  by (induction m) auto
-
 lemma length_flatten_multiset: 
   assumes "finite M"
   shows "length (flatten_multiset M) = Finite_Set.fold (\<lambda> (t, m) y. y + (the_enat m)) 0 M"
-  using length_fold[of "flatten_multiset M"] by (simp add: fold_flatten_multiset assms comp_fun_commute.intro iter_f_len)
+  using length_fold[of "flatten_multiset M"] fold_flatten_multiset[of M "(\<lambda>_ n. n + 1)" 0]
+  by (simp add: fold_flatten_multiset assms comp_fun_commute.intro) (meson add.commute)
+
+lemma other_evals_unchanged:
+  assumes elem_group: "drop b elem = k"
+  and diff_group: "x \<noteq> meval_trm f elem"
+  shows "(x, y) \<in> group_multiset k b f (insert elem X) \<longleftrightarrow> (x, y) \<in> group_multiset k b f X"
+proof
+  define old_group where [simp]: "old_group = group k b X"
+  define new_group where [simp]: "new_group = group k b (X \<union> {elem})"
+  have aux1: "\<And>x. x \<noteq> meval_trm f elem \<Longrightarrow> Set.filter (\<lambda>xa. meval_trm f xa = x) new_group = Set.filter (\<lambda>xa. meval_trm f xa = x) old_group" by auto
+  assume assm: "(x, y) \<in> group_multiset k b f (insert elem X)"
+  then have x_old_eval: "x \<in> meval_trm f ` old_group" using diff_group by(auto simp: Let_def)
+  have "y = ecard (Set.filter (\<lambda>xa. meval_trm f xa = x) new_group)" using assm by(auto simp: Let_def)
+  then have "y =  ecard (Set.filter (\<lambda>xa. meval_trm f xa = x) old_group)" using aux1 diff_group by auto
+  then show "(x, y) \<in>  group_multiset k b f X" using x_old_eval by (auto simp: Let_def)
+next
+  define old_group where [simp]: "old_group = group k b X"
+  define new_group where [simp]: "new_group = group k b (X \<union> {elem})"
+  have aux1: "\<And>x. x \<noteq> meval_trm f elem \<Longrightarrow> Set.filter (\<lambda>xa. meval_trm f xa = x) new_group = Set.filter (\<lambda>xa. meval_trm f xa = x) old_group" by auto
+  assume assm: "(x, y) \<in>  group_multiset k b f X"
+  then have x_old_eval: "x \<in> meval_trm f ` old_group" by(auto simp: Let_def)
+  have "y = ecard (Set.filter (\<lambda>xa. meval_trm f xa = x) old_group)" using assm by(auto simp: Let_def)
+  then have "y =  ecard (Set.filter (\<lambda>xa. meval_trm f xa = x) new_group)" using aux1 diff_group by auto
+  then show "(x, y) \<in> group_multiset k b f (insert elem X)" using x_old_eval by (auto simp: Let_def)
+qed
+
+lemma multiset_new_term_insert:
+  assumes elem_group: "drop b elem = k"
+  and new_term_eval: "Set.filter (\<lambda>x. meval_trm f x = meval_trm f elem) (group k b X) = {}"
+  shows "group_multiset k b f (insert elem X) = insert (meval_trm f elem, 1) (group_multiset k b f X)"
+proof -
+  define updated_data where [simp]: "updated_data = X \<union> {elem}"
+  define old_group where [simp]: "old_group = group k b X"
+  define new_group where [simp]: "new_group = group k b updated_data"
+  define old_evals where "old_evals = meval_trm f ` old_group"
+  have aux: "Set.filter (\<lambda>x. drop b x = k) (insert elem X) = insert elem old_group" using elem_group by auto
+  have aux1: "\<And>x. x \<noteq> meval_trm f elem \<Longrightarrow> Set.filter (\<lambda>xa. meval_trm f xa = x) new_group = Set.filter (\<lambda>xa. meval_trm f xa = x) old_group" by auto
+  have aux2: "meval_trm f elem \<notin> old_evals" using new_term_eval by (auto simp: old_evals_def)
+  moreover have "Set.filter (\<lambda>x. meval_trm f x = meval_trm f elem) new_group = {elem}" using new_term_eval elem_group by auto
+  moreover have "ecard {elem} = 1" using enat_1 by (auto simp:ecard_def)
+  moreover have "(\<lambda>x. (x, ecard (Set.filter (\<lambda>xa. meval_trm f xa = x) new_group))) ` old_evals = 
+                 (\<lambda>x. (x, ecard (Set.filter (\<lambda>xa. meval_trm f xa = x) old_group))) ` old_evals"
+    using other_evals_unchanged by (metis (mono_tags, lifting) aux1 aux2 image_cong)
+  ultimately show "group_multiset k b f (insert elem X) = insert (meval_trm f elem, 1) (group_multiset k b f X)" using aux
+    by(simp add:Let_def old_evals_def)
+qed
+
+lemma multiset_old_term_insert:
+  assumes elem_group: "drop b elem = k"
+  and old_term_eval: "Set.filter (\<lambda>x. meval_trm f x = meval_trm f elem) (group k b X) \<noteq> {}"
+  and old_val: "(meval_trm f elem, y) \<in> group_multiset k b f X" 
+  and disjoint: "elem \<notin> X"
+  and finite: "finite X"
+  shows "group_multiset k b f (insert elem X) = 
+         insert (meval_trm f elem, y + 1) ((group_multiset k b f X) - {(meval_trm f elem, y)})"
+proof (rule set_eqI, rule iffI)
+  fix x
+  assume x_in_M: "x \<in> group_multiset k b f (insert elem X)"
+  then obtain t v where x_def: "x = (t, v)" by fastforce
+  define updated_data where [simp]: "updated_data = X \<union> {elem}"
+  define old_group where [simp]: "old_group = group k b X"
+  define new_group where [simp]: "new_group = group k b updated_data"
+  define old_evals where "old_evals = meval_trm f ` old_group"
+  have group_ins: "new_group = insert elem old_group" using elem_group by auto
+  have y_card: "y = ecard (Set.filter (\<lambda>xa. meval_trm f xa = meval_trm f elem) old_group)" using old_val by (auto simp: Let_def)
+  moreover have "Set.filter (\<lambda>xa. meval_trm f xa = meval_trm f elem) (insert elem (Set.filter (\<lambda>x. drop b x = k) X)) =
+                 insert elem  (Set.filter (\<lambda>xa. meval_trm f xa = meval_trm f elem) (Set.filter (\<lambda>x. drop b x = k) X))" by auto
+  moreover have "elem \<notin> Set.filter (\<lambda>xa. meval_trm f xa = meval_trm f elem) (Set.filter (\<lambda>x. drop b x = k) X)" by (meson Set.member_filter disjoint)
+  ultimately have correct_card: "y + 1 = ecard (Set.filter (\<lambda>xa. meval_trm f xa = meval_trm f elem) new_group)" 
+    using eSuc_enat plus_1_eSuc(2) group_ins by(auto simp: ecard_def) 
+  then have aux1: "(meval_trm f elem, y + 1) \<in> group_multiset k b f (insert elem X)" using group_ins by (auto simp:Let_def)
+  have aux2: "(meval_trm f elem, y) \<notin> group_multiset k b f (insert elem X)" 
+    using unique_term_multiset[of "meval_trm f elem" "y + 1" k b f updated_data y] aux1 y_card
+    by(simp add:Let_def) (meson ecard_def finite_filter finite valid_maggaux.simps)
+  show "x \<in> insert (meval_trm f elem, y + 1) ((group_multiset k b f X) - {(meval_trm f elem, y)})"
+  proof (cases "t = meval_trm f elem")
+    case True
+    then have "v = y + 1" using x_in_M x_def aux1 using unique_term_multiset by blast
+    then show ?thesis using x_def x_in_M True by auto
+  next
+    case False
+    then show ?thesis using other_evals_unchanged 
+      by (metis Pair_inject Set.member_remove elem_group insertI2 x_def x_in_M)
+  qed
+next
+  fix x
+  assume x_in_oldM: "x \<in> insert (meval_trm f elem, y + 1) ((group_multiset k b f X) - {(meval_trm f elem, y)})"
+  then obtain t v where x_def: "x = (t, v)" by force
+  define updated_data where [simp]: "updated_data = X \<union> {elem}"
+  define old_group where [simp]: "old_group = group k b X"
+  define new_group where [simp]: "new_group = group k b updated_data"
+  define old_evals where "old_evals = meval_trm f ` old_group"
+  have group_ins: "new_group = insert elem old_group" using elem_group by auto
+  have y_card: "y = ecard (Set.filter (\<lambda>xa. meval_trm f xa = meval_trm f elem) old_group)" using old_val by (auto simp: Let_def)
+  moreover have "Set.filter (\<lambda>xa. meval_trm f xa = meval_trm f elem) (insert elem (Set.filter (\<lambda>x. drop b x = k) X)) =
+                 insert elem  (Set.filter (\<lambda>xa. meval_trm f xa = meval_trm f elem) (Set.filter (\<lambda>x. drop b x = k) X))" by auto
+  moreover have "elem \<notin> Set.filter (\<lambda>xa. meval_trm f xa = meval_trm f elem) (Set.filter (\<lambda>x. drop b x = k) X)" by (meson Set.member_filter disjoint)
+  ultimately have correct_card: "y + 1 = ecard (Set.filter (\<lambda>xa. meval_trm f xa = meval_trm f elem) new_group)" 
+    using eSuc_enat plus_1_eSuc(2) group_ins by(auto simp: ecard_def) 
+  then have aux1: "(meval_trm f elem, y + 1) \<in> group_multiset k b f (insert elem X)" using group_ins by (auto simp:Let_def)
+  show "x \<in> group_multiset k b f (insert elem X)" 
+  proof (cases "t = meval_trm f elem")
+    case True
+    then have "v = y + 1" using x_in_oldM x_def by (metis DiffE insertE old.prod.inject old_val singleton_iff unique_term_multiset)
+    then show ?thesis using True aux1 x_def by blast
+  next
+    case False
+    then show ?thesis by (metis DiffD1 elem_group insertE old.prod.inject other_evals_unchanged x_def x_in_oldM)
+  qed
+qed  
 
 lemma valid_insert_cnt_unfolded: 
   assumes valid_before: "valid_maggaux \<lparr>aggargs_cols = cols, aggargs_n = n, aggargs_g0 = g0, aggargs_y = y, aggargs_\<omega> = \<omega>, aggargs_b = b, aggargs_f = f\<rparr> (CntAux m) X" 
-  and correct_type: "type_restr \<lparr>aggargs_cols = cols, aggargs_n = n, aggargs_g0 = g0, aggargs_y = y, aggargs_\<omega> = \<omega>, aggargs_b = b, aggargs_f = f\<rparr> {elem}"
   and disjoint: "elem \<notin> X"
 shows "valid_maggaux \<lparr>aggargs_cols = cols, aggargs_n = n, aggargs_g0 = g0, aggargs_y = y, aggargs_\<omega> = \<omega>, aggargs_b = b, aggargs_f = f\<rparr> 
-        (CntAux (insert_cnt \<lparr>aggargs_cols = cols, aggargs_n = n, aggargs_g0 = g0, aggargs_y = y, aggargs_\<omega> = \<omega>, aggargs_b = b, aggargs_f = f\<rparr> m elem)) (X \<union> {elem})"
+        (CntAux (insert_cnt \<lparr>aggargs_cols = cols, aggargs_n = n, aggargs_g0 = g0, aggargs_y = y, aggargs_\<omega> = \<omega>, aggargs_b = b, aggargs_f = f\<rparr> elem m)) (X \<union> {elem})"
 proof - 
-  define updated_map where "updated_map = insert_cnt \<lparr>aggargs_cols = cols, aggargs_n = n, aggargs_g0 = g0, aggargs_y = y, aggargs_\<omega> = \<omega>, aggargs_b = b, aggargs_f = f\<rparr> m elem"
-  define updated_data where "updated_data = X \<union> {elem}"
+  define updated_map where [simp]: "updated_map = insert_cnt \<lparr>aggargs_cols = cols, aggargs_n = n, aggargs_g0 = g0, aggargs_y = y, aggargs_\<omega> = \<omega>, aggargs_b = b, aggargs_f = f\<rparr> elem m"
+  define updated_data where [simp]: "updated_data = X \<union> {elem}"
   interpret comp_fun_commute "\<lambda>(t, m) y. y + the_enat m" 
     by(unfold_locales) auto
-  have valid_finite: "finite updated_data" using valid_before by (auto simp:updated_data_def)
+  have valid_finite: "finite updated_data" using valid_before by auto
   have valid_key_invariant: "\<And>k. k \<in> (drop b) ` updated_data \<longleftrightarrow> k \<in> Mapping.keys updated_map"
   proof (rule iffI)
     fix k
     assume assm: "k \<in> (drop b) ` updated_data"
     show "k \<in>  Mapping.keys updated_map"
       using valid_before assm
-      unfolding updated_map_def updated_data_def
-      by (cases "k \<in> (drop b) ` X") (auto simp: valid_aggmap_def Let_def split:option.splits)
+      by (cases "k \<in> (drop b) ` X") (auto simp: Let_def split:option.splits)
   next
     fix k
     assume assm: "k \<in> Mapping.keys updated_map"
     show "k \<in> (drop b) ` updated_data"
       using valid_before assm
-      unfolding updated_map_def updated_data_def
-      by (cases "k \<in> Mapping.keys m") (auto simp: valid_aggmap_def Let_def split:option.splits)
+      by (cases "k \<in> Mapping.keys m") (auto simp: Let_def split:option.splits)
   qed
   have valid_value_invariant: "\<And>k. k \<in> Mapping.keys updated_map \<longrightarrow> Mapping.lookup updated_map k = 
           (let group = Set.filter (\<lambda>x. drop b x = k) updated_data;
@@ -204,10 +335,11 @@ proof -
           in Some (length (flatten_multiset M)))"
   proof rule
     fix k
-    define group where "group = Set.filter (\<lambda>x. drop b x = k) updated_data"
-    define M where "M = (\<lambda>y. (y, ecard (Set.filter (\<lambda>x. meval_trm f x = y) group))) ` meval_trm f ` group"
-    define old_group where "old_group = Set.filter (\<lambda>x. drop b x = k) X"
-    define old_M where "old_M = (\<lambda>y. (y, ecard (Set.filter (\<lambda>x. meval_trm f x = y) old_group))) ` meval_trm f ` old_group"
+    define group where [simp]: "group = Set.filter (\<lambda>x. drop b x = k) updated_data"
+    define M where [simp]: "M = (\<lambda>y. (y, ecard (Set.filter (\<lambda>x. meval_trm f x = y) group))) ` meval_trm f ` group"
+    define old_group where [simp]: "old_group = Set.filter (\<lambda>x. drop b x = k) X"
+    define old_M where [simp]: "old_M = (\<lambda>y. (y, ecard (Set.filter (\<lambda>x. meval_trm f x = y) old_group))) ` meval_trm f ` old_group"
+    define old_evals where "old_evals = meval_trm f ` old_group"
     assume assm: "k \<in> Mapping.keys updated_map"
     show "Mapping.lookup updated_map k = 
           (let group = Set.filter (\<lambda>x. drop b x = k) updated_data;
@@ -216,30 +348,128 @@ proof -
     proof (cases "k \<in> Mapping.keys m")
       case False
       then have map_val: "Mapping.lookup updated_map k = Some 1" 
-        using assm by (auto simp: updated_map_def keys_is_none_rep Let_def lookup_update' split:option.splits)
+        using assm by (auto simp: keys_is_none_rep Let_def lookup_update' split:option.splits)
       have "drop b elem = k" 
         using assm False 
-        by(auto simp: updated_map_def Let_def split:option.splits)
+        by(auto simp: Let_def split:option.splits)
       then have group_single_elem: "group = {elem}" 
         using False valid_before image_iff
-        by(fastforce simp: group_def updated_data_def valid_aggmap_def)
+        by fastforce
       then have "M = insert (meval_trm f elem, enat 1) {}"
         using group_single_elem unfolding M_def Set.filter_def ecard_def by (auto cong: conj_cong)
       then have "length(flatten_multiset M) = 1" 
         using length_flatten_multiset[of M] Finite_Set.comp_fun_commute.fold_insert by(auto)
-      then show ?thesis using map_val by (simp add: M_def local.group_def)
+      then show ?thesis using map_val by simp
     next
       case True
-      then show ?thesis sorry
-        
+      then have in_map: "k \<in> Mapping.keys m" by auto
+      show ?thesis
+      proof(cases "drop b elem = k")
+        case True
+        then have elem_group: "drop b elem = k" by auto
+        then have newgroup_def: "group = insert elem old_group" by auto
+        have both_finite: "finite old_M \<and> finite M" using valid_before by auto
+        have "length(flatten_multiset(M)) = length(flatten_multiset(old_M)) + 1"
+        proof(cases "Set.filter (\<lambda>x. meval_trm f x = meval_trm f elem) old_group = {}")
+          case True
+          then have "M = insert (meval_trm f elem, 1) old_M" using multiset_new_term_insert elem_group by(simp add: Let_def)
+          moreover have "(meval_trm f elem, 1) \<notin> old_M" using True by auto
+          ultimately show ?thesis using both_finite by (auto simp:length_flatten_multiset one_enat_def)
+        next
+          case False
+          then obtain y where y_def: "(meval_trm f elem, y) \<in> old_M" 
+            by (smt (z3) Collect_empty_eq Set.filter_def image_eqI old_M_def)
+          then obtain i where i_def: "y = enat i" 
+            by (smt (z3) Pair_inject ecard_def finite_filter image_iff old_M_def old_group_def valid_before valid_maggaux.simps)
+          have finite_remove: "finite (old_M - {(meval_trm f elem, y)})" using both_finite finite_Diff  by (auto simp: Set.remove_def)
+          have finite_insert: "finite (insert (meval_trm f elem, y) old_M)" using both_finite by blast
+          have M_insert_remove_def: "M = insert (meval_trm f elem, y + 1) (old_M - {(meval_trm f elem, y)})" 
+            using multiset_old_term_insert[of b elem k f X y] elem_group False y_def valid_before disjoint
+            by(simp only: M_def old_M_def group_def old_group_def updated_data_def group_multiset_def Let_def Optimized_Agg.group_def) auto          
+          then have aux: "length(flatten_multiset(insert (meval_trm f elem, y) old_M)) = length(flatten_multiset(old_M - {(meval_trm f elem, y)})) + i" 
+            using both_finite finite_insert finite_remove 
+            Finite_Set.comp_fun_commute.fold_insert_remove[of "\<lambda>(t, m) y. y + the_enat m" old_M 0 "(meval_trm f elem, y)"]
+            by (simp only: length_flatten_multiset) (metis comp_fun_commute_axioms i_def old.prod.case the_enat.simps)
+          have "(meval_trm f elem, y + 1) \<notin> old_M - {(meval_trm f elem, y)}" using y_def by auto
+          then show ?thesis using both_finite finite_remove M_insert_remove_def i_def Finite_Set.comp_fun_commute.fold_insert[of "\<lambda>(t, m) y. y + the_enat m" "old_M - {(meval_trm f elem, y)}" "(meval_trm f elem, y + 1)" 0]
+            by (metis (mono_tags, lifting) aux case_prod_conv comp_fun_commute_axioms group_cancel.add1 insert_absorb length_flatten_multiset one_enat_def plus_enat_simps(1) the_enat.simps y_def)
+        qed
+        moreover obtain len where len_def: "Mapping.lookup m k = Some len \<and> len = length(flatten_multiset(old_M))" 
+          using valid_before in_map by auto metis
+        then have "Mapping.lookup updated_map k = Some (len + 1)" by (simp add: elem_group lookup_update)
+        ultimately show ?thesis by (simp add: len_def)
+      next
+        case False
+        then have same_group: "group = old_group" by auto
+        then have "M = old_M" by auto
+        then have "Mapping.lookup updated_map k = Mapping.lookup m k" 
+          using False by (auto split:option.splits simp:Let_def lookup_update')
+        then show ?thesis using valid_before same_group in_map 
+          by (auto simp: Let_def)
+      qed
     qed
   qed
   show ?thesis using valid_value_invariant valid_key_invariant valid_finite valid_before
-    by (auto simp add:updated_data_def valid_aggmap_def updated_map_def group_multiset_def Let_def)
+    by (auto simp add: Let_def)
 qed
 
+lemma valid_insert_maggaux_unfolded: 
+  "valid_maggaux \<lparr>aggargs_cols = cols, aggargs_n = n, aggargs_g0 = g0, aggargs_y = y, aggargs_\<omega> = \<omega>, aggargs_b = b, aggargs_f = f\<rparr> aux X \<Longrightarrow>
+  finite Y \<Longrightarrow>
+  X \<inter> Y = {} \<Longrightarrow>
+  valid_maggaux \<lparr>aggargs_cols = cols, aggargs_n = n, aggargs_g0 = g0, aggargs_y = y, aggargs_\<omega> = \<omega>, aggargs_b = b, aggargs_f = f\<rparr> 
+  (insert_maggaux \<lparr>aggargs_cols = cols, aggargs_n = n, aggargs_g0 = g0, aggargs_y = y, aggargs_\<omega> = \<omega>, aggargs_b = b, aggargs_f = f\<rparr> Y aux) (X \<union> Y)" 
+proof(induction aux)
+  case (CntAux m)
+  have disjoint: "X \<inter> Y = {}" using CntAux by auto
+  have finite_y: "finite Y" using CntAux by auto
+  then show ?case using disjoint
+  proof(induction Y)
+    case empty
+    then show ?case using CntAux by auto
+  next
+    case (insert x F)
+    define args where "args = \<lparr>aggargs_cols = cols, aggargs_n = n, aggargs_g0 = g0, aggargs_y = y, aggargs_\<omega> = \<omega>, aggargs_b = b, aggargs_f = f\<rparr>"
+    interpret comp_fun_commute "insert_cnt args"
+      using insert_cnt_comm by unfold_locales auto
+    obtain intermediate_map where intermediate_map_def: "CntAux intermediate_map = insert_maggaux args F (CntAux m)" by auto
+    have valid_a: "valid_maggaux args (CntAux (insert_cnt args x intermediate_map)) (X \<union> F \<union> {x})" 
+      using insert valid_insert_cnt_unfolded disjoint Un_iff args_def intermediate_map_def by (metis disjoint_insert(1))
+    then have "Finite_Set.fold (insert_cnt args) m (insert x F) = insert_cnt args x (Finite_Set.fold (insert_cnt args) m F)"
+      using  Finite_Set.comp_fun_commute.fold_insert[of "insert_cnt args" F x m] insert by auto
+    moreover have "CntAux (Finite_Set.fold (insert_cnt args) m F) = CntAux intermediate_map"
+      by(auto simp:intermediate_map_def)
+    ultimately have "insert_maggaux args (insert x F) (CntAux m) = CntAux (insert_cnt args x intermediate_map)"
+      using  Finite_Set.comp_fun_commute.fold_insert[of "insert_cnt args" F x m]
+      by auto
+    then have "valid_maggaux args (insert_maggaux args (insert x F) (aggaux.CntAux m)) (X \<union> insert x F)"
+      using valid_a
+      by auto
+    then show ?case
+      by (auto simp: args_def)
+  qed
+next
+case (SumAux x)
+  then show ?case sorry
+next
+  case (MinAux x)
+  then show ?case sorry
+next
+  case (MaxAux x)
+  then show ?case sorry
+next
+  case (MedAux x)
+  then show ?case sorry
+qed
+
+lemma valid_insert_maggaux: "valid_maggaux args aux X \<Longrightarrow> finite Y \<Longrightarrow>
+    table (aggargs_b args + aggargs_n args) (aggargs_cols args) Y \<Longrightarrow>
+    type_restr args Y \<Longrightarrow> X \<inter> Y = {} \<Longrightarrow>
+    valid_maggaux args (insert_maggaux args Y aux) (X \<union> Y)"
+  using valid_insert_maggaux_unfolded by (cases args) fast
+
 lemma valid_aggmap_empty_data: "valid_aggmap g b f m X \<Longrightarrow> X = {} \<longleftrightarrow> Mapping.keys m = {}"
-  by (auto simp:valid_aggmap_def)
+  by auto
 
 lemma flatten_multiset_not_empty: 
   assumes valid_map: "valid_aggmap g b f m X"
@@ -247,30 +477,28 @@ lemma flatten_multiset_not_empty:
   and in_map: "k \<in> Mapping.keys m"
   shows "flatten_multiset (group_multiset k b f X) \<noteq> []"
 proof -
-  define M where "M = group_multiset k b f X"
+  define M where [simp]: "M = group_multiset k b f X"
   obtain c where c_def: "ID ccompare = Some (c :: (event_data \<times> enat) comparator)" 
     by (simp add: ID_def ccompare_prod_def ccompare_event_data_def ccompare_enat_def split:if_splits option.splits)
   note c = ID_ccompare'[OF c_def] 
   note c_class = comparator.linorder[OF c]
-  define M_list where "M_list = linorder.sorted_list_of_set (le_of_comp c) M"
-  obtain elem where elem_prop: "elem \<in> X \<and> drop b elem = k" using in_map valid_map imageE[of k "drop b" X] by (auto simp: valid_aggmap_def)
+  define M_list where [simp]: "M_list = linorder.sorted_list_of_set (le_of_comp c) M"
+  obtain elem where elem_prop: "elem \<in> X \<and> drop b elem = k" using in_map valid_map imageE[of k "drop b" X] by auto
   then obtain m where m_prop: "(meval_trm f elem, m) \<in> M" 
-    by (auto simp: group_multiset_def Let_def valid_aggmap_def M_def) fastforce
-  define group where "group = Set.filter (\<lambda>x. meval_trm f x = meval_trm f elem) (Set.filter (\<lambda>x. drop b x = k) X)"
-  then have "elem \<in> group" using elem_prop by (auto simp: group_def)
-  moreover have finite_g: "finite group" using finite by (auto simp: group_def)
-  ultimately have "ecard group \<noteq> 0" by (auto simp:ecard_def zero_enat_def)
+    by (auto simp: Let_def) fastforce
+  define group where [simp]: "group = Set.filter (\<lambda>x. meval_trm f x = meval_trm f elem) (Set.filter (\<lambda>x. drop b x = k) X)"
+  have "ecard group \<noteq> 0" using finite elem_prop by (auto simp:ecard_def zero_enat_def) 
   then have m_pos: "m > 0 \<and> m \<noteq> \<infinity>" 
-    using elem_prop m_prop finite_g  by (auto simp: M_def group_multiset_def Let_def group_def ecard_def)
+    using elem_prop m_prop finite  by (auto simp: Let_def ecard_def)
   then have "the_enat m > 0"
     apply(auto simp: the_enat_def)
     using enat_0_iff(1) by blast
   then obtain n where n_def: "the_enat m = Suc n" using gr0_implies_Suc by auto
-  have finite_m: "finite M" using finite by (auto simp: M_def group_multiset_def Let_def)
+  have finite_m: "finite M" using finite by (auto simp: Let_def)
   then have "(meval_trm f elem, m) \<in> set (linorder.sorted_list_of_set (le_of_comp c) M)"
     using m_prop linorder.set_sorted_list_of_set[OF c_class] by auto
   then show ?thesis 
-    using finite_m n_def by (simp add:flatten_multiset_def csorted_list_of_set_def c_def M_def) force
+    using finite_m n_def by (simp add:flatten_multiset_def csorted_list_of_set_def c_def) force
 qed
   
 lemma valid_result_maggaux_unfolded: "valid_maggaux \<lparr>aggargs_cols = cols, aggargs_n = n, aggargs_g0 = g0, aggargs_y = y, aggargs_\<omega> = \<omega>, aggargs_b = b, aggargs_f = f\<rparr> aux X
@@ -282,10 +510,10 @@ proof(induction aux)
   proof (cases "g0 \<and> X = {}")
     case True
     then show ?thesis unfolding eval_aggargs_def eval_agg_def using SumAux
-      by (auto simp add: valid_aggmap_def)
+      by auto
   next
     case False
-    then have assm_map: "\<not>(g0 \<and> Mapping.keys m = {})" using valid_aggmap_empty_data[of _ b f m X] SumAux by force
+    then have assm_map: "\<not>(g0 \<and> Mapping.keys m = {})" using valid_aggmap_empty_data[of _ b f m X] SumAux by fastforce
     have assm_reg: "\<not>(g0 \<and> X = {})" using False by auto
     show ?thesis
     proof (cases "fst \<omega> = Formula.Agg_Sum")
@@ -297,14 +525,14 @@ proof(induction aux)
       then obtain k where k_assm: "k \<in> Mapping.keys m \<and> result = (case Mapping.lookup m k of 
                                                       Some (_, agg_sum) \<Rightarrow> k[y:=Some agg_sum]
                                                     | None \<Rightarrow> k)" using assm_map True by auto
-      define group where "group = Set.filter (\<lambda>x. drop b x = k) X"
-      define M where "M = (\<lambda>y. (y, ecard (Set.filter (\<lambda>x. meval_trm f x = y) group))) ` meval_trm f ` group"
+      define group where [simp]: "group = Set.filter (\<lambda>x. drop b x = k) X"
+      define M where [simp]: "M = (\<lambda>y. (y, ecard (Set.filter (\<lambda>x. meval_trm f x = y) group))) ` meval_trm f ` group"
       have "Mapping.lookup m k = Some (length (flatten_multiset M), foldl plus (snd \<omega>) (flatten_multiset M))" 
-        using SumAux k_assm True by (simp add: M_def group_def Let_def lookup_default_def valid_aggmap_def group_multiset_def)
+        using SumAux k_assm True by (simp add: Let_def lookup_default_def)
       then have "result = k[y:= Some (eval_agg_op \<omega> M)]" 
-        using k_assm True by auto (metis eval_agg_op.simps(4) prod.collapse)
+        using k_assm True by auto (metis (no_types, lifting) eval_agg_op.simps(4) prod.exhaust_sel)
       then show "result \<in> eval_aggargs \<lparr>aggargs_cols = cols, aggargs_n = n, aggargs_g0 = g0, aggargs_y = y, aggargs_\<omega> = \<omega>, aggargs_b = b, aggargs_f = f\<rparr> X"
-        using k_assm SumAux by (auto simp add: M_def group_def Let_def eval_agg_def eval_aggargs_def valid_aggmap_def)
+        using k_assm SumAux by (auto simp add: Let_def eval_agg_def eval_aggargs_def)
     next
       fix result
       assume "result \<in> eval_aggargs \<lparr>aggargs_cols = cols, aggargs_n = n, aggargs_g0 = g0, aggargs_y = y, aggargs_\<omega> = \<omega>, aggargs_b = b, aggargs_f = f\<rparr> X"
@@ -312,12 +540,12 @@ proof(induction aux)
                                                                    M = (\<lambda>y. (y, ecard (Set.filter (\<lambda>x. meval_trm f x = y) group))) ` meval_trm f ` group
                                                                  in k[y:=Some (eval_agg_op \<omega> M)]))" 
         unfolding eval_aggargs_def eval_agg_def empty_table_def using False by auto
-      define group where "group = Set.filter (\<lambda>x. drop b x = k) X"
-      define M where "M = (\<lambda>y. (y, ecard (Set.filter (\<lambda>x. meval_trm f x = y) group))) ` meval_trm f ` group"
+      define group where [simp]: "group = Set.filter (\<lambda>x. drop b x = k) X"
+      define M where [simp]: "M = (\<lambda>y. (y, ecard (Set.filter (\<lambda>x. meval_trm f x = y) group))) ` meval_trm f ` group"
       have key_in_map: "k \<in> Mapping.keys m"
-        using SumAux by (auto simp add:valid_aggmap_def) (metis k_assm)
+        using SumAux by auto (metis k_assm)
       then have "Mapping.lookup m k = Some (length (flatten_multiset M), foldl plus (snd \<omega>) (flatten_multiset M))"
-        using SumAux True by (simp add: M_def group_def Let_def lookup_default_def valid_aggmap_def group_multiset_def)
+        using SumAux True by (simp add: Let_def lookup_default_def)
       then have "result = (case Mapping.lookup m k of 
                             Some (_, agg_sum) \<Rightarrow> k[y:=Some agg_sum]
                           | None \<Rightarrow> k)"
@@ -337,18 +565,18 @@ proof(induction aux)
       then obtain k where k_assm: "k \<in> Mapping.keys m \<and> result = (case Mapping.lookup m k of 
                                                       Some (cnt, agg_sum) \<Rightarrow> k[y:=Some (EFloat ((double_of_event_data agg_sum) / (double_of_int cnt)))]
                                                     | None \<Rightarrow> k)" using assm_map agg_type by auto
-      define group where "group = Set.filter (\<lambda>x. drop b x = k) X"
-      define M where "M = (\<lambda>y. (y, ecard (Set.filter (\<lambda>x. meval_trm f x = y) group))) ` meval_trm f ` group"
+      define group where [simp]: "group = Set.filter (\<lambda>x. drop b x = k) X"
+      define M where [simp]: "M = (\<lambda>y. (y, ecard (Set.filter (\<lambda>x. meval_trm f x = y) group))) ` meval_trm f ` group"
       have not_empty: "flatten_multiset M \<noteq> []" 
         using flatten_multiset_not_empty[of _ b f m X k] SumAux k_assm False 
-        by (auto simp: Let_def M_def group_multiset_def group_def)
+        by (auto simp: Let_def) force
       have "Mapping.lookup m k = Some (length (flatten_multiset M), foldl plus (EInt 0) (flatten_multiset M))" 
-        using SumAux k_assm agg_type by (simp add: M_def group_def Let_def lookup_default_def valid_aggmap_def group_multiset_def)
+        using SumAux k_assm agg_type by (simp add: Let_def lookup_default_def)
       then have "result = k[y:= Some (eval_agg_op \<omega> M)]" 
         using k_assm agg_type not_empty SumAux aux_def
-        by(auto simp add:valid_aggmap_def Let_def M_def group_def group_multiset_def split:list.splits)
+        by(auto simp add: Let_def split:list.splits)
       then show "result \<in> eval_aggargs \<lparr>aggargs_cols = cols, aggargs_n = n, aggargs_g0 = g0, aggargs_y = y, aggargs_\<omega> = \<omega>, aggargs_b = b, aggargs_f = f\<rparr> X"
-        using k_assm SumAux by (auto simp add: M_def group_def Let_def eval_agg_def eval_aggargs_def valid_aggmap_def)
+        using k_assm SumAux by (auto simp add: Let_def eval_agg_def eval_aggargs_def)
     next
       fix result
       assume "result \<in> eval_aggargs \<lparr>aggargs_cols = cols, aggargs_n = n, aggargs_g0 = g0, aggargs_y = y, aggargs_\<omega> = \<omega>, aggargs_b = b, aggargs_f = f\<rparr> X"
@@ -356,17 +584,17 @@ proof(induction aux)
                                                                    M = (\<lambda>y. (y, ecard (Set.filter (\<lambda>x. meval_trm f x = y) group))) ` meval_trm f ` group
                                                                  in k[y:=Some (eval_agg_op \<omega> M)]))" 
         unfolding eval_aggargs_def eval_agg_def empty_table_def using assm_reg by auto
-      define group where "group = Set.filter (\<lambda>x. drop b x = k) X"
-      define M where "M = (\<lambda>y. (y, ecard (Set.filter (\<lambda>x. meval_trm f x = y) group))) ` meval_trm f ` group"
+      define group where [simp]: "group = Set.filter (\<lambda>x. drop b x = k) X"
+      define M where [simp]: "M = (\<lambda>y. (y, ecard (Set.filter (\<lambda>x. meval_trm f x = y) group))) ` meval_trm f ` group"
       have "k \<in> Mapping.keys m" using k_assm SumAux 
       by (metis (no_types, lifting) aggaux.simps(27) valid_aggmap_def valid_maggaux.simps)
       then have not_empty: "flatten_multiset M \<noteq> []" 
         using flatten_multiset_not_empty[of _ b f m X k] SumAux k_assm False 
         unfolding group_multiset_def Let_def M_def group_def by fastforce
       have key_in_map: "k \<in> Mapping.keys m"
-        using SumAux by (auto simp add:valid_aggmap_def) (metis k_assm)
+        using SumAux by auto (metis k_assm)
       then have "Mapping.lookup m k = Some (length (flatten_multiset M), foldl plus (EInt 0) (flatten_multiset M))"
-        using SumAux False by (simp add: M_def group_def Let_def lookup_default_def valid_aggmap_def group_multiset_def)
+        using SumAux False by (simp add: Let_def lookup_default_def)
       then have "result = (case Mapping.lookup m k of 
                              Some (cnt, agg_sum) \<Rightarrow> k[y:=Some (EFloat ((double_of_event_data agg_sum) / (double_of_int cnt)))]
                           | None \<Rightarrow> k)"
@@ -394,10 +622,10 @@ next
     case(True)
     then show ?thesis 
       unfolding eval_aggargs_def eval_agg_def
-      using CntAux by (auto simp add: valid_aggmap_def)
+      using CntAux by auto
   next
     case(False)
-    then have assm_map: "\<not>(g0 \<and> Mapping.keys m = {})" using CntAux by (auto simp add: valid_aggmap_def)
+    then have assm_map: "\<not>(g0 \<and> Mapping.keys m = {})" using CntAux by auto
     show ?thesis
     proof (rule set_eqI, rule iffI)
       fix result
@@ -409,17 +637,17 @@ next
       then obtain k where k_assm: "k \<in> Mapping.keys m \<and> result = (case Mapping.lookup m k of
                                                       Some i \<Rightarrow> k[y:=Some (EInt (integer_of_int i))]
                                                     | None \<Rightarrow> k)" by blast
-      define group where "group = Set.filter (\<lambda>x. drop b x = k) X"
-      define M where "M = (\<lambda>y. (y, ecard (Set.filter (\<lambda>x. meval_trm f x = y) group))) ` meval_trm f ` group"
+      define group where [simp]: "group = Set.filter (\<lambda>x. drop b x = k) X"
+      define M where [simp]: "M = (\<lambda>y. (y, ecard (Set.filter (\<lambda>x. meval_trm f x = y) group))) ` meval_trm f ` group"
       have "Mapping.lookup m k = Some (length (flatten_multiset M))" 
         using CntAux k_assm 
-        by (simp add: M_def group_def Let_def lookup_default_def valid_aggmap_def group_multiset_def)
+        by (simp add: Let_def lookup_default_def)
       then have "result = k[y:= Some (eval_agg_op \<omega> M)]" 
         using k_assm agg_type 
         by (metis eval_agg_op.simps(1) option.simps(5) prod.collapse)
       then show "result \<in> eval_aggargs \<lparr>aggargs_cols = cols, aggargs_n = n, aggargs_g0 = g0, aggargs_y = y, aggargs_\<omega> = \<omega>, aggargs_b = b, aggargs_f = f\<rparr> X"
         using k_assm CntAux
-        by (auto simp add: M_def group_def Let_def eval_agg_def eval_aggargs_def valid_aggmap_def)
+        by (auto simp add: Let_def eval_agg_def eval_aggargs_def)
     next
       fix result
       assume "result \<in> eval_aggargs \<lparr>aggargs_cols = cols, aggargs_n = n, aggargs_g0 = g0, aggargs_y = y, aggargs_\<omega> = \<omega>, aggargs_b = b, aggargs_f = f\<rparr> X"
@@ -431,13 +659,11 @@ next
       then obtain k where k_assm: "(k \<in> (drop b) ` X \<and> result = (let group = Set.filter (\<lambda>x. drop b x = k) X;
                                                                    M = (\<lambda>y. (y, ecard (Set.filter (\<lambda>x. meval_trm f x = y) group))) ` meval_trm f ` group
                                                                  in k[y:=Some (eval_agg_op \<omega> M)]))" by blast
-      define group where "group = Set.filter (\<lambda>x. drop b x = k) X"
-      define M where "M = (\<lambda>y. (y, ecard (Set.filter (\<lambda>x. meval_trm f x = y) group))) ` meval_trm f ` group"
-      have key_in_map: "k \<in> Mapping.keys m"
-        using CntAux k_assm by (auto simp add:valid_aggmap_def)
-      then have "Mapping.lookup m k = Some (length (flatten_multiset M))"
-        using CntAux 
-        by (simp add: M_def group_def Let_def lookup_default_def valid_aggmap_def group_multiset_def)
+      define group where [simp]: "group = Set.filter (\<lambda>x. drop b x = k) X"
+      define M where [simp]: "M = (\<lambda>y. (y, ecard (Set.filter (\<lambda>x. meval_trm f x = y) group))) ` meval_trm f ` group"
+      have "Mapping.lookup m k = Some (length (flatten_multiset M))"
+        using CntAux k_assm
+        by (simp add: Let_def lookup_default_def)
       then have "result = (case Mapping.lookup m k of
                              Some i \<Rightarrow> k[y:=Some (EInt (integer_of_int i))]
                            | None \<Rightarrow> k)"
@@ -445,7 +671,7 @@ next
         unfolding M_def group_def
         by (metis (no_types, lifting) eval_agg_op.simps(1) option.simps(5) prod.collapse)
       then show  "result \<in> result_maggaux \<lparr>aggargs_cols = cols, aggargs_n = n, aggargs_g0 = g0, aggargs_y = y, aggargs_\<omega> = \<omega>, aggargs_b = b, aggargs_f = f\<rparr> (CntAux m)"
-        using key_in_map by auto
+        using CntAux k_assm by auto
     qed
   qed
 qed
